src/model/Thread.v
@@ -16,7 +16,6 @@ Require Import Time.
 Require Import View.
 Require Import BoolMap.
 Require Import Promises.
-Require Import Reserves.
 Require Import Cell.
 Require Import Memory.
 Require Import TView.
@@ -86,7 +85,6 @@ Qed.
 Module Thread.
   Section Thread.
     Variable (lang: language).
-    Variable (reserved: TimeMap.t).
 
     Structure t := mk {
       state: (Language.state lang);
@@ -94,55 +92,40 @@ Module Thread.
       global: Global.t;
     }.
 
-    Variant step: forall (pf: bool) (e: ThreadEvent.t) (th1 th2: t), Prop :=
+    Variant step: forall (e: ThreadEvent.t) (th1 th2: t), Prop :=
     | step_internal
         e st lc1 gl1 lc2 gl2
         (LOCAL: Local.internal_step e lc1 gl1 lc2 gl2):
-      step false e (mk st lc1 gl1) (mk st lc2 gl2)
+      step e (mk st lc1 gl1) (mk st lc2 gl2)
     | step_program
-        e sth1 lc1 gl1 sth2 lc2 gl2
-        (STATE: Language.step lang (ThreadEvent.get_program_event e) sth1 sth2)
-        (LOCAL: Local.program_step reserved e lc1 gl1 lc2 gl2):
-        step true e (mk sth1 lc1 gl1) (mk sth2 lc2 gl2)
+        e st1 lc1 gl1 st2 lc2 gl2
+        (STATE: Language.step lang (ThreadEvent.get_program_event e) st1 st2)
+        (LOCAL: Local.program_step e lc1 gl1 lc2 gl2):
+      step e (mk st1 lc1 gl1) (mk st2 lc2 gl2)
     .
-    #[local] Hint Constructors step: core.
+    Hint Constructors step: core.
 
-    Variant step_allpf (e:ThreadEvent.t) (th1 th2:t): Prop :=
-    | step_nopf_intro
-        pf
-        (STEP: step pf e th1 th2)
-    .
-    #[local] Hint Constructors step_allpf: core.
-
-    Lemma allpf pf: step pf <3= step_allpf.
-    Proof.
-      i. econs. eauto.
-    Qed.
-
-    Definition pf_tau_step := tau (step true).
-    Hint Unfold pf_tau_step: core.
-
-    Definition tau_step := tau step_allpf.
+    Definition tau_step := tau step.
     Hint Unfold tau_step: core.
 
-    Definition all_step := union step_allpf.
+    Definition all_step := union step.
     Hint Unfold all_step: core.
 
-    Variant opt_step: forall (pf: bool) (e:ThreadEvent.t) (th1 th2:t), Prop :=
+    Variant opt_step: forall (e:ThreadEvent.t) (th1 th2:t), Prop :=
       | step_none
           th:
-        opt_step true ThreadEvent.silent th th
+        opt_step ThreadEvent.silent th th
       | step_some
-          pf e th1 th2
-          (STEP: step pf e th1 th2):
-        opt_step pf e th1 th2
+          e th1 th2
+          (STEP: step e th1 th2):
+        opt_step e th1 th2
     .
-    #[local] Hint Constructors opt_step: core.
+    Hint Constructors opt_step: core.
 
     Lemma tau_opt_tau
-          th1 th2 th3 pf e
+          th1 th2 th3 e
           (STEPS: rtc tau_step th1 th2)
-          (STEP: opt_step pf e th2 th3)
+          (STEP: opt_step e th2 th3)
           (EVENT: ThreadEvent.get_machine_event e = MachineEvent.silent):
       rtc tau_step th1 th3.
     Proof.
@@ -152,33 +135,42 @@ Module Thread.
     Qed.
 
     Lemma tau_opt_all
-          th1 th2 th3 pf e
+          th1 th2 th3 e
           (STEPS: rtc tau_step th1 th2)
-          (STEP: opt_step pf e th2 th3):
+          (STEP: opt_step e th2 th3):
       rtc all_step th1 th3.
     Proof.
       induction STEPS.
       - inv STEP; eauto.
       - exploit IHSTEPS; eauto. i.
         econs 2; eauto.
-        inv H. inv TSTEP. econs. econs. eauto.
+        inv H. econs. eauto.
     Qed.
 
 
+    (* consistency *)
+
     Variant steps_failure (th1: t): Prop :=
-    | steps_failure_intro
-        pf e th2 th3
-        (STEPS: rtc tau_step th1 th2)
-        (STEP_FAILURE: step pf e th2 th3)
-        (EVENT_FAILURE: ThreadEvent.get_machine_event e = MachineEvent.failure)
+      | steps_failure_intro
+          e th2 th3
+          (STEPS: rtc tau_step th1 th2)
+          (STEP_FAILURE: step e th2 th3)
+          (EVENT_FAILURE: ThreadEvent.get_machine_event e = MachineEvent.failure)
     .
+
+    Definition consistent (th: t): Prop :=
+      forall gl_cap (CAP: Global.cap (global th) gl_cap),
+        (<<FAILURE: steps_failure (Thread.mk (state th) (local th) gl_cap)>>) \/
+        exists th2,
+          (<<STEPS: rtc tau_step (Thread.mk (state th) (local th) gl_cap) th2>>) /\
+          (<<PROMISES: Local.promises (Thread.local th2) = BoolMap.bot>>).
 
 
     (* step_future *)
 
     Lemma step_future
-          pf e th1 th2
-          (STEP: step pf e th1 th2)
+          e th1 th2
+          (STEP: step e th1 th2)
           (LC_WF1: Local.wf (local th1) (global th1))
           (GL_WF1: Global.wf (global th1)):
       <<LC_WF2: Local.wf (local th2) (global th2)>> /\
@@ -187,13 +179,13 @@ Module Thread.
       <<GL_FUTURE: Global.future (global th1) (global th2)>>.
     Proof.
       inv STEP; ss.
-      - eapply Local.internal_step_future; eauto.
-      - eapply Local.program_step_future; eauto.
+      - eauto using Local.internal_step_future.
+      - eauto using Local.program_step_future.
     Qed.
 
     Lemma opt_step_future
-          pf e th1 th2
-          (STEP: opt_step pf e th1 th2)
+          e th1 th2
+          (STEP: opt_step e th1 th2)
           (LC_WF1: Local.wf (local th1) (global th1))
           (GL_WF1: Global.wf (global th1)):
       <<LC_WF2: Local.wf (local th2) (global th2)>> /\
@@ -201,9 +193,8 @@ Module Thread.
       <<TVIEW_FUTURE: TView.le (Local.tview (local th1)) (Local.tview (local th2))>> /\
       <<GL_FUTURE: Global.future (global th1) (global th2)>>.
     Proof.
-      inv STEP.
-      - esplits; eauto; refl.
-      - eapply step_future; eauto.
+      inv STEP; eauto using step_future.
+      esplits; eauto; refl.
     Qed.
 
     Lemma rtc_all_step_future
@@ -216,10 +207,9 @@ Module Thread.
       <<TVIEW_FUTURE: TView.le (Local.tview (local th1)) (Local.tview (local th2))>> /\
       <<GL_FUTURE: Global.future (global th1) (global th2)>>.
     Proof.
-      revert LC_WF1. induction STEP.
-      - i. splits; ss; refl.
-      - i. inv H. inv USTEP.
-        exploit step_future; eauto. i. des.
+      revert LC_WF1. induction STEP; i.
+      - splits; ss; refl.
+      - inv H. exploit step_future; eauto. i. des.
         exploit IHSTEP; eauto. i. des.
         splits; ss; etrans; eauto.
     Qed.
@@ -239,45 +229,12 @@ Module Thread.
       apply tau_union.
     Qed.
 
-    Lemma step_nonpf_future
-          e th1 th2
-          (STEP: step false e th1 th2)
-          (LC_WF1: Local.wf (local th1) (global th1))
-          (GL_WF1: Global.wf (global th1)):
-      <<LC_WF2: Local.wf (local th2) (global th2)>> /\
-      <<GL_WF2: Global.wf (global th2)>> /\
-      <<TVIEW_FUTURE: TView.le (Local.tview (local th1)) (Local.tview (local th2))>> /\
-      <<GL_FUTURE: Global.future (global th1) (global th2)>> /\
-      <<STATE: (state th1) = (state th2)>>.
-    Proof.
-      exploit step_future; eauto. i. des.
-      inv STEP. inv LOCAL; esplits; ss.
-    Qed.
-
-    Lemma rtc_step_nonpf_future
-          th1 th2
-          (STEP: rtc (union (step false)) th1 th2)
-          (LC_WF1: Local.wf (local th1) (global th1))
-          (GL_WF1: Global.wf (global th1)):
-      <<LC_WF2: Local.wf (local th2) (global th2)>> /\
-      <<GL_WF2: Global.wf (global th2)>> /\
-      <<TVIEW_FUTURE: TView.le (Local.tview (local th1)) (Local.tview (local th2))>> /\
-      <<GL_FUTURE: Global.future (global th1) (global th2)>> /\
-      <<STATE: (state th1) = (state th2)>>.
-    Proof.
-      revert LC_WF1. induction STEP.
-      - i. splits; ss; refl.
-      - inv H. i. exploit step_nonpf_future; eauto. i. des.
-        exploit IHSTEP; eauto. i. des.
-        splits; ss; etrans; eauto.
-    Qed.
-
 
     (* step_inhabited *)
 
     Lemma step_inhabited
-          pf e th1 th2
-          (STEP: step pf e th1 th2)
+          e th1 th2
+          (STEP: step e th1 th2)
           (INHABITED1: Memory.inhabited (Global.memory (global th1))):
       <<INHABITED2: Memory.inhabited (Global.memory (global th2))>>.
     Proof.
@@ -290,8 +247,8 @@ Module Thread.
     (* step_disjoint *)
 
     Lemma step_disjoint
-          pf e th1 th2 lc
-          (STEP: step pf e th1 th2)
+          e th1 th2 lc
+          (STEP: step e th1 th2)
           (DISJOINTH1: Local.disjoint (local th1) lc)
           (LC_WF: Local.wf lc (global th1)):
       <<DISJOINTH2: Local.disjoint (local th2) lc>> /\
@@ -303,8 +260,8 @@ Module Thread.
     Qed.
 
     Lemma opt_step_disjoint
-          pf e th1 th2 lc
-          (STEP: opt_step pf e th1 th2)
+          e th1 th2 lc
+          (STEP: opt_step e th1 th2)
           (DISJOINTH1: Local.disjoint (local th1) lc)
           (LC_WF: Local.wf lc (global th1)):
       <<DISJOINTH2: Local.disjoint (local th2) lc>> /\
@@ -324,9 +281,7 @@ Module Thread.
       <<LC_WF: Local.wf lc (global th2)>>.
     Proof.
       revert DISJOINTH1 LC_WF. induction STEP; eauto. i.
-      inv H. inv USTEP.
-      exploit step_disjoint; eauto. i. des.
-      exploit IHSTEP; eauto.
+      inv H. exploit step_disjoint; eauto. i. des. eauto.
     Qed.
 
     Lemma rtc_tau_step_disjoint
@@ -344,27 +299,18 @@ Module Thread.
 
     Lemma program_step_promises
           e th1 th2
-          (STEP: Thread.step true e th1 th2):
+          (STEP: Thread.step e th1 th2)
+          (EVENT: ThreadEvent.is_program e):
       BoolMap.le (Local.promises (local th2)) (Local.promises (local th1)) /\
-      BoolMap.le (Global.reserves (global th2)) (Global.reserves (global th1)).
+      BoolMap.le (Global.promises (global th2)) (Global.promises (global th1)).
     Proof.
-      inv STEP. ss.
+      inv STEP; try by (inv LOCAL; ss).
       eapply Local.program_step_promises; eauto.
     Qed.
 
-    Lemma program_step_reserves
-          e th1 th2
-          (STEP: Thread.step true e th1 th2):
-      Local.reserves (local th1) = Local.reserves (local th2) /\
-      Global.reserves (global th1) = Global.reserves (global th2).
-    Proof.
-      inv STEP. ss.
-      eapply Local.program_step_reserves; eauto.
-    Qed.
-
     Lemma step_promises_minus
-          pf e th1 th2
-          (STEP: step pf e th1 th2):
+          e th1 th2
+          (STEP: step e th1 th2):
       BoolMap.minus (Global.promises (Thread.global th1)) (Local.promises (Thread.local th1)) =
       BoolMap.minus (Global.promises (Thread.global th2)) (Local.promises (Thread.local th2)).
     Proof.
@@ -379,8 +325,7 @@ Module Thread.
       BoolMap.minus (Global.promises (Thread.global th1)) (Local.promises (Thread.local th1)) =
       BoolMap.minus (Global.promises (Thread.global th2)) (Local.promises (Thread.local th2)).
     Proof.
-      induction STEPS; ss.
-      inv H. inv USTEP.
+      induction STEPS; ss. inv H.
       exploit step_promises_minus; eauto. i. congr.
     Qed.
 
@@ -394,72 +339,9 @@ Module Thread.
       eapply rtc_implies; try exact STEPS.
       apply tau_union.
     Qed.
-
-    Lemma step_reserves_minus
-          pf e th1 th2
-          (STEP: step pf e th1 th2):
-      BoolMap.minus (Global.reserves (Thread.global th1)) (Local.reserves (Thread.local th1)) =
-      BoolMap.minus (Global.reserves (Thread.global th2)) (Local.reserves (Thread.local th2)).
-    Proof.
-      inv STEP; s.
-      - eapply Local.internal_step_reserves_minus; eauto.
-      - eapply Local.program_step_reserves_minus; eauto.
-    Qed.
-
-    Lemma rtc_all_step_reserves_minus
-          th1 th2
-          (STEPS: rtc all_step th1 th2):
-      BoolMap.minus (Global.reserves (Thread.global th1)) (Local.reserves (Thread.local th1)) =
-      BoolMap.minus (Global.reserves (Thread.global th2)) (Local.reserves (Thread.local th2)).
-    Proof.
-      induction STEPS; ss.
-      inv H. inv USTEP.
-      exploit step_reserves_minus; eauto. i. congr.
-    Qed.
-
-    Lemma rtc_tau_step_reserves_minus
-          th1 th2
-          (STEPS: rtc tau_step th1 th2):
-      BoolMap.minus (Global.reserves (Thread.global th1)) (Local.reserves (Thread.local th1)) =
-      BoolMap.minus (Global.reserves (Thread.global th2)) (Local.reserves (Thread.local th2)).
-    Proof.
-      apply rtc_all_step_reserves_minus.
-      eapply rtc_implies; try exact STEPS.
-      apply tau_union.
-    Qed.
   End Thread.
-
-
-  (* consistency *)
-
-  Definition fully_reserved {lang: language} (th: t lang): t lang :=
-    mk lang (state th) (local th) (Global.fully_reserved (global th)).
-
-  Lemma fully_reserved_wf
-        lang (th: t lang)
-        (LC_WF: Local.wf (local th) (global th))
-        (GL_WF: Global.wf (global th)):
-    (<<LC_WF: Local.wf (local (fully_reserved th)) (global (fully_reserved th))>>) /\
-    (<<GL_WF: Global.wf (global (fully_reserved th))>>).
-  Proof.
-    exploit Local.fully_reserved_wf; eauto. i.
-    exploit Global.fully_reserved_wf; eauto.
-  Qed.
-
-  Variant consistent {lang: language} (th: t lang): Prop :=
-    | consistent_failure
-        (FAILURE: @steps_failure lang (Memory.max_timemap (Global.memory (global th)))
-                                 (fully_reserved th))
-    | consistent_promises
-        th2
-        (STEPS: rtc (@tau_step lang (Memory.max_timemap (Global.memory (global th))))
-                    (fully_reserved th) th2)
-        (PROMISES: Local.promises (Thread.local th2) = BoolMap.bot)
-  .
 End Thread.
 #[export] Hint Constructors Thread.step: core.
-#[export] Hint Constructors Thread.step_allpf: core.
 #[export] Hint Constructors Thread.opt_step: core.
 #[export] Hint Constructors Thread.steps_failure: core.
-#[export] Hint Unfold Thread.fully_reserved: core.
-#[export] Hint Constructors Thread.consistent: core.
+#[export] Hint Unfold Thread.consistent: core.
